# I
#### Week I Contents
- Introduction
- Analyzing Algorithms: The 2-d Maxima Problem
- Summations and Analyzing Programs with Loops
##

_Before you implement, first be sure you have a good design._

#### Design Strategy Basics
1. Design a few solutions from a mathematical perspective
2. Prune selection by consideration of practical matters
3. Prototype the best designs
4. Run on data sets

##

## The 2-d Maxima Problem
_Example:  I want the fastest and cheapest car possible_
- Fastest may not be cheapest and vice versa
- Fast cheap car dominates the expensive slow car
- Given collection of cars, we need to list those not dominated by any others
- Formally: 
    ```
        p - point in 2-d space
        p.x and p.y are coordinates
        
        p = (p.x, p.y)
        
        p is dominated by q if {
            p.x <= q.x
            &&
            p.y <= q.y
        }
    ```
- P = {p1, p2, ... , pN} is maximal if not dominated by any other point in P
- **Brute force** way to find the **maxima** is testing each point against every other point

## Running Time Analysis
- Measuring run time and space for an algorithm

### Worst-case time
- Maximum running time over all legal inputs of size _n_
- _n_ = size
- _I_ = input
- |_I_| = length
- _T(I)_ = running time
- _T(n) = maxT(I)_

### Average-case time
- weight sum of average-case running times
- _p(I)_ = probability of this input
- _T(n) = SUM(p(I)T(I))_

## 

#### Proving Recursive Functions are Correct
- Iterative function:
```
int triangular(int n){
	int result = 0;
	for (int i = 1; i <= n; i ++) {
		result += i;
	}
	return result;
}
```
- Recursive version:
```
// precondition: n >= 1
int triangular(int n) {
	if (n == 1) {
		return n
	}
	return triangular(n--) + n;
}
// postcondition: return n(n + 1)/ 2
```
- Proof by induction:
    ```
    Base case:  n=1
        n(n+1)/2
        1(1+1)/2 = 1
        which is what is returned in base case
    ```
    ```
    Inductive case:
        assume true for n=k-1
        prove it is true for n=k, when n>1
        
        return value = triangular(k-1) + k
        = (k-1)*(k-1+1) / 2 + k
        = (k^2 - k + 2k) / 2
        = k(k+1)/2
        QED.
    ```
##
#### Determining When One Algorithm Becomes More Efficient

     